WIP

NuBasicAbstractors.thy
@@ -47,7 +47,10 @@ lemma [\<nu>intro]: "\<nu>ShrIdentical N sid \<Longrightarrow> \<nu>ShrIdentical
 lemma [\<nu>intro]: "\<nu>Disposable \<tort_lbrace>x \<tycolon> N\<tort_rbrace> \<Longrightarrow> \<nu>Disposable \<tort_lbrace>x \<tycolon> (N \<^bold>w\<^bold>h\<^bold>e\<^bold>r\<^bold>e S)\<tort_rbrace>" unfolding \<nu>Disposable_def by simp
 lemma [\<nu>intro]: "\<^bold>p\<^bold>r\<^bold>e\<^bold>m\<^bold>i\<^bold>s\<^bold>e z \<in> S \<Longrightarrow> \<nu>Zero N z \<Longrightarrow> \<nu>Zero (N \<^bold>w\<^bold>h\<^bold>e\<^bold>r\<^bold>e S) z" unfolding \<nu>Zero_def Premise_def by simp
 
-lemma [simp]: "\<tort_lbrace>x \<tycolon> N \<^bold>w\<^bold>h\<^bold>e\<^bold>r\<^bold>e SchemaTag P\<tort_rbrace> = (\<tort_lbrace>x \<tycolon> N\<tort_rbrace> \<addition> (x \<in> P))" unfolding SchemaTag_def by auto
+definition SchemaCondition (infixl "<where''>" 80) where "SchemaCondition = NuRefine"
+
+lemma [simp]: "\<tort_lbrace>x \<tycolon> N <where'> P\<tort_rbrace> = (\<tort_lbrace>x \<tycolon> N\<tort_rbrace> \<addition> (x \<in> P))" unfolding SchemaCondition_def by auto
+lemma SchemaCondition_simp: "\<tort_lbrace> x \<tycolon> N <where'> P\<tort_rbrace> = \<tort_lbrace> x \<tycolon> N \<^bold>w\<^bold>h\<^bold>e\<^bold>r\<^bold>e P\<tort_rbrace>" unfolding SchemaCondition_def by auto
 
 subsubsection \<open>Down Lifting\<close>
 
