NuInstructions.thy
@@ -90,22 +90,21 @@ specification ("op_while_WF")
   \<Longrightarrow> \<^bold>p\<^bold>r\<^bold>o\<^bold>c op_while_WF TYPE('c) brC brB \<blangle> (R \<heavy_comma> x \<tycolon> X) \<flower> W \<longmapsto> (R \<heavy_comma> - P \<tycolon> \<^bold>s\<^bold>o\<^bold>m\<^bold>e X) \<flower> W \<brangle>"
   apply (rule exI) using op_crash by auto
 
-consts op_while :: "'c itself \<Rightarrow> (('x::lrep) \<times> ('r::stack) \<flower> ('w::register_collection) \<Rightarrow> (('x \<times> 1 word) \<times> 'r \<flower> 'w) state)
+consts op_while :: "'c itself \<Rightarrow> (('x::lrep) \<times> ('r::stack) \<flower> ('w::register_collection) \<Rightarrow> ((1 word \<times> 'x) \<times> 'r \<flower> 'w) state)
   \<Rightarrow> ('x \<times> 'r \<flower> 'w \<Rightarrow> ('x \<times> 'r \<flower> 'w) state) \<Rightarrow> ('x \<times> 'r \<flower> 'w \<Rightarrow> ('x \<times> 'r \<flower> 'w) state)"
 specification ("op_while")
   i_while_raw_\<nu>proc[simplified PremiseHOL ParamHOL]: "
   ParamHOL P
-  \<Longrightarrow> (\<And>x1. \<^bold>p\<^bold>r\<^bold>o\<^bold>c brC \<blangle> (R \<heavy_comma> (x1::'c) \<tycolon> X) \<flower> W \<longmapsto> (R \<heavy_comma> {(y, y \<in> P) |y. True } \<tycolon> \<^bold>s\<^bold>o\<^bold>m\<^bold>e (X \<nuFusion> \<bool>)) \<flower> W \<brangle>)
+  \<Longrightarrow> (\<And>x1. \<^bold>p\<^bold>r\<^bold>o\<^bold>c brC \<blangle> (R \<heavy_comma> (x1::'c) \<tycolon> X) \<flower> W \<longmapsto> (R \<heavy_comma> {(y \<in> P, y) |y. True } \<tycolon> \<^bold>s\<^bold>o\<^bold>m\<^bold>e (\<bool> \<nuFusion> X)) \<flower> W \<brangle>)
   \<Longrightarrow> (\<And>x2. \<^bold>p\<^bold>r\<^bold>o\<^bold>c brB \<blangle> (R \<heavy_comma> x2 \<tycolon> (X \<^bold>w\<^bold>h\<^bold>e\<^bold>r\<^bold>e P)) \<flower> W \<longmapsto> (R \<heavy_comma> UNIV \<tycolon> \<^bold>s\<^bold>o\<^bold>m\<^bold>e X) \<flower> W \<brangle>)
   \<Longrightarrow> \<^bold>p\<^bold>r\<^bold>o\<^bold>c op_while TYPE('c) brC brB \<blangle> (R \<heavy_comma> x \<tycolon> X) \<flower> W \<longmapsto> (R \<heavy_comma> - P \<tycolon> \<^bold>s\<^bold>o\<^bold>m\<^bold>e X) \<flower> W \<brangle>"
   apply (rule exI) using op_crash by auto
 
 proc' i_while: \<open>(R \<heavy_comma> x \<tycolon> X) \<flower> W\<close> \<longmapsto> \<open>(R \<heavy_comma> - P \<tycolon> \<^bold>s\<^bold>o\<^bold>m\<^bold>e (X <schema> sch)) \<flower> W\<close>
   requires "\<^bold>p\<^bold>a\<^bold>r\<^bold>a\<^bold>m sch" and "\<^bold>p\<^bold>a\<^bold>r\<^bold>a\<^bold>m P" and [THEN someI_ex, intro]: "\<exists>y. sch y = x" 
-    and brC: \<open>(\<And>x1. \<^bold>p\<^bold>r\<^bold>o\<^bold>c brC \<blangle> (R \<heavy_comma> x1 \<tycolon> X <schema> sch) \<flower> W \<longmapsto> (R \<heavy_comma> {(y, y \<in> P) |y. True } \<tycolon> \<^bold>s\<^bold>o\<^bold>m\<^bold>e (X <schema> sch \<nuFusion> \<bool>)) \<flower> W \<brangle>)\<close>
-    and brB: \<open>(\<And>x2. \<^bold>p\<^bold>r\<^bold>o\<^bold>c brB \<blangle> (R \<heavy_comma> x2 \<tycolon> (X <schema> sch \<^bold>w\<^bold>h\<^bold>e\<^bold>r\<^bold>e SchemaTag P)) \<flower> W \<longmapsto> (R \<heavy_comma> UNIV \<tycolon> \<^bold>s\<^bold>o\<^bold>m\<^bold>e (X <schema> sch)) \<flower> W \<brangle>)\<close>
-  \<nu>have A: "SchemaTag P = P" unfolding SchemaTag_def by simp
-  \<bullet> cast i_schema sch  i_while_raw P \<Longleftarrow> brC \<Longleftarrow> brB[simplified A] finish
+    and brC: \<open>(\<And>x1. \<^bold>p\<^bold>r\<^bold>o\<^bold>c brC \<blangle> (R \<heavy_comma> x1 \<tycolon> X <schema> sch) \<flower> W \<longmapsto> (R \<heavy_comma> { (y \<in> P, y) |y. True } \<tycolon> \<^bold>s\<^bold>o\<^bold>m\<^bold>e (\<bool> \<nuFusion> X <schema> sch)) \<flower> W \<brangle>)\<close>
+    and brB: \<open>(\<And>x2. \<^bold>p\<^bold>r\<^bold>o\<^bold>c brB \<blangle> (R \<heavy_comma> x2 \<tycolon> (X <schema> sch <where'> P)) \<flower> W \<longmapsto> (R \<heavy_comma> UNIV \<tycolon> \<^bold>s\<^bold>o\<^bold>m\<^bold>e (X <schema> sch)) \<flower> W \<brangle>)\<close>
+  \<bullet> cast i_schema sch  i_while_raw P \<Longleftarrow> brC \<Longleftarrow> brB[simplified SchemaCondition_simp] finish
 
 \<nu>processor while 110 \<open>\<^bold>c\<^bold>u\<^bold>r\<^bold>r\<^bold>e\<^bold>n\<^bold>t blk \<^bold>r\<^bold>e\<^bold>s\<^bold>u\<^bold>l\<^bold>t\<^bold>s \<^bold>i\<^bold>n (T \<flower> W)\<close> \<open>fn ctx => fn meta => let open Parse Scan NuHelp NuBasics in
   $$$ "while" |-- vars -- option ($$$ "in" |-- term) -- ($$$ "subj" |-- term) >> (fn ((vars, schema), subj) => fn _ =>
@@ -127,11 +126,6 @@ proc' i_while: \<open>(R \<heavy_comma> x \<tycolon> X) \<flower> W\<close> \<lo
           |> NuSys.set_param ctx schema |> NuSys.set_param ctx subj
   end
 ) end\<close>
-
-proc AA: \<open>i \<tycolon> \<nat>[32]\<heavy_comma>  zp \<left_fish_tail> adr \<R_arr_tail> z \<left_fish_tail> i \<tycolon> Ref \<nat>[32]\<close> \<longmapsto> \<open>i + j \<tycolon> \<nat>[32]\<close>
-  \<bullet> i \<leftarrow> v while i j in \<open>(i, zp \<left_fish_tail> adr \<R_arr_tail> z \<left_fish_tail> j)\<close> subj \<open>i < j\<close> \<medium_left_bracket> \<bullet>
-
-thm i_while_\<nu>compilation
 
 subsubsection \<open>recursion\<close>
 
@@ -584,125 +578,8 @@ proc i_pop_refs[simplified length_greater_0_conv, \<nu>overload pop]:
   requires [used]: "0 < length xs"
   \<nu>have A[simp]: "take 1 xs = [hd xs]" by (simp add: One_nat_def take_Suc)
   \<nu>have B[simp]: "drop 1 xs = tl xs" by (simp add: One_nat_def drop_Suc) 
-  \<bullet> \<leftarrow> v \<open>1 \<tycolon> \<nat>[32]\<close> split affirm by linarith
+  \<bullet> \<leftarrow> v \<open>1 \<tycolon> \<nat>[32]\<close> split affirm by linarith \<bullet>
   finish
 
   
-
-section \<open>Tests\<close>
-
-abbreviation "FullRef N \<equiv> Ref N <down-lift> (\<lambda>raw. case raw of a \<R_arr_tail> x \<Rightarrow> Gz \<left_fish_tail> a \<R_arr_tail> Gi 0 \<left_fish_tail> x)"
-abbreviation "Array N \<equiv> RefS N <down-lift> (\<lambda>raw. case raw of a \<R_arr_tail> x \<Rightarrow> Gz \<left_fish_tail> a \<R_arr_tail> Gi 0 \<left_fish_tail> x)"
-
-proc' [\<nu>overload pop]: \<open>R\<heavy_comma> (seg |+ i) \<R_arr_tail> xs \<tycolon> Array N\<close> \<longmapsto> \<open>R\<heavy_comma> (seg |+ i + 1) \<R_arr_tail> tl xs \<tycolon> Array N\<heavy_comma> (seg |+ i) \<R_arr_tail> hd xs \<tycolon> FullRef N\<close>
-  requires [simp]: "xs \<noteq> []"
-  \<bullet> pop finish
-
-
-lemma [\<nu>overload pop]: "\<^bold>p\<^bold>r\<^bold>e\<^bold>m\<^bold>i\<^bold>s\<^bold>e xs \<noteq> [] \<Longrightarrow> \<^bold>p\<^bold>r\<^bold>o\<^bold>c i_pop_refs \<blangle> R\<heavy_comma> (seg |+ i) \<R_arr_tail> xs \<tycolon> Array N
-      \<longmapsto>  R\<heavy_comma> (seg |+ i + 1) \<R_arr_tail> tl xs \<tycolon> Array N\<heavy_comma> (seg |+ i) \<R_arr_tail> hd xs \<tycolon> FullRef N \<brangle>" sorry
-
-abbreviation "permuted l1 l2 \<equiv> set l1 = set l2"
-
-declare pair_forall[simp]
-
-proc qsort: \<open> (seg |+ i) \<R_arr_tail> xs \<tycolon> Array \<nat>[32]\<heavy_comma> n \<tycolon> \<nat>[32]\<close>
-  \<longmapsto> \<open>{ (seg |+ i) \<R_arr_tail> ys | ys. permuted xs ys \<and> sorted ys } \<tycolon> \<^bold>s\<^bold>o\<^bold>m\<^bold>e (Array \<nat>[32])\<close>
-  requires "length xs = n"
-  \<bullet> \<leftarrow> (v,n) pr recursion \<open>(\<lambda>x. case x of ((seg |+ i) \<R_arr_tail> xs, n) \<Rightarrow>
-        { (seg |+ i) \<R_arr_tail> ys | ys. permuted xs ys \<and> sorted ys })\<close> \<open>\<^bold>s\<^bold>o\<^bold>m\<^bold>e (Array \<nat>[32])\<close>
-  \<medium_left_bracket> (g_\<nu>proc) \<nu>obtain seg i xs n  where [simp]: "x' = ((seg |+ i) \<R_arr_tail> xs, n)"
-  by (metis memadr.exhaust object.exhaust old.prod.exhaust) \<bullet>
-  \<nu>obtain seg i xs n  where B[simp]: "x' = ((seg |+ i) \<R_arr_tail> xs, n)"
-by (metis memadr.exhaust object.exhaust old.prod.exhaust) \<bullet>
-  \<bullet> dpr \<rightarrow> (xs, n) n 0 = if 
-  \<nu>debug note g_\<nu>proc
-
-ML \<open>Locale.get_locales @{theory}\<close>
-ML \<open>val ctx = Locale.init "NuPrim.ceq_lrep" @{theory}
-val x = Assumption.all_prems_of ctx\<close>
-
-(* schematic_goal [simplified, simplified \<nu>post_construct]:
-  "\<^bold>c\<^bold>o\<^bold>n\<^bold>s\<^bold>t\<^bold>r\<^bold>u\<^bold>c\<^bold>t (233 \<tycolon> \<nat>[32], ((copy_reg::((32 word register \<times> 32 word register), (32 word register \<times> 32 word register), (32 word) register, 32 word register) address \<Rightarrow> (32 word, nat) typing)) (address_left address_here)
-+ (233 \<tycolon>  \<nat>[32])) \<^bold>b\<^bold>y \<^bold>p\<^bold>r\<^bold>o\<^bold>c ?f \<blangle>((?Z1::(?'a::lrep) set) \<flower> \<^bold>r\<^bold>e\<^bold>g\<^bold>i\<^bold>s\<^bold>t\<^bold>e\<^bold>r A = \<tort_lbrace> 16 \<tycolon> \<nat>[32]\<tort_rbrace> and_ty \<^bold>r\<^bold>e\<^bold>g\<^bold>i\<^bold>s\<^bold>t\<^bold>e\<^bold>r B = \<tort_lbrace> 0 \<tycolon> \<nat>[32] \<tort_rbrace>) \<longmapsto> (?Z2::(?'b::lrep) set) \<brangle>"
-  by  (\<nu>resolve \<nu>intro (\<nu>intro'))  *)
-
-
-
-
-fun fib :: "nat \<Rightarrow> nat"
-  where "fib x = (if x = 0 then 1 else if x = 1 then 1 else fib (x-1) + fib (x-2))"
-
-proc fibx : "x \<tycolon> \<nat>[32]" \<longmapsto> "fib x \<tycolon> \<nat>\<^sup>r[32]"
-  \<bullet> x recursion fib \<open>\<nat>\<^sup>r[32]\<close> less_than \<medium_left_bracket> (g_\<nu>proc)
-  \<bullet> \<rightarrow> x x 0 = if \<medium_left_bracket> \<bullet> \<open>1\<tycolon>\<nat>\<^sup>r[32]\<close> \<medium_right_bracket> \<medium_left_bracket> (c0[used])
-      \<bullet> x 1 = if \<medium_left_bracket> \<bullet> \<open>1\<tycolon>\<nat>\<^sup>r[32]\<close> \<medium_right_bracket> \<medium_left_bracket> (c1[used]) \<bullet> x 1 - g \<rightarrow> f1 x 2 - g \<rightarrow> f2 f1 f2 + \<medium_right_bracket>
-  \<medium_right_bracket> \<medium_right_bracket>
-  finish
-
-  thm fibx_\<nu>proc
-
-fun ackman :: "(nat \<times> nat) \<Rightarrow> nat"
-  where "ackman (0,n) = Suc n"
-  | "ackman (Suc m, 0) = ackman (m,1)"
-  | "ackman (Suc m, Suc n) = ackman (m, ackman (Suc m, n))"
-
-thm begin_proc_ctx
-proc ackman : "(x \<tycolon> \<nat>[32], y \<tycolon> \<nat>[32])" \<longmapsto> "ackman (x,y) \<tycolon> \<nat>[32]" if cond: "ackman (x,y) < 2^32"
-  \<bullet> x y pr cast where \<open>{xy. ackman xy < 2^32}\<close> affirm using cond by simp
-  \<bullet> recursion ackman \<open>\<nat>[32]\<close> \<open>less_than <*lex*> less_than\<close> \<medium_left_bracket> (g_\<nu>proc)
-  \<nu>obtain m n where th1[simp]: "x' = (m,n)" by (cases x')
-  \<bullet> cast E \<Longrightarrow> th2[used] \<bullet> dpr \<rightarrow> (m,n) m 0 = if \<medium_left_bracket> \<bullet> n 1 + \<medium_right_bracket> \<medium_left_bracket> \<bullet> m 1 -
-  \<bullet> n 0 = if \<medium_left_bracket> \<bullet> 1 pr 
-  \<bullet> cast where \<open>{xy. ackman xy < 2^32}\<close> affirm apply (cases m) by auto
-  \<bullet> g \<medium_right_bracket> \<medium_left_bracket> \<bullet> m n 1 - pr
-\<bullet> cast where \<open>{xy. ackman xy < 2^32}\<close> affirm apply (cases m; cases n) by auto
-  note c
-  \<nu>debug 
-  note c
-
-end
-
-definition [simp]:"difference x y = (if x < y then y - x else x - y)"
-xproc diff : "(x \<tycolon> \<nat>[32], y \<tycolon> \<nat>[32])" \<longmapsto> "(difference x y \<tycolon> \<nat>[32])"
-  \<bullet> x while \<open>{x. 0 < x}\<close> Id less_than \<medium_left_bracket> \<bullet> \<rightarrow> a a 0 a < pr \<medium_right_bracket> \<medium_left_bracket> \<bullet> cast E \<Longrightarrow> th1[used] \<bullet> 1 -  \<medium_right_bracket>
-  \<bullet> cast E \<nu>choose a where "some = a" by auto
-  \<bullet> \<Longrightarrow> th1[simp] drop_fact th1
-  \<bullet> drop x y < if \<medium_left_bracket> \<bullet> y x - \<medium_right_bracket> \<medium_left_bracket> \<bullet> x y - \<medium_right_bracket>
-  finish
-
-end
-
-proc add2 : "(( x \<tycolon> \<nat>[32]) named x, y \<tycolon> \<nat>[32])" \<longmapsto> "(x + x + y \<tycolon> \<nat>[32])"
-  if "x < 100" and "y < 100"
-  \<nu>have x[used]: "x < 100 \<and> y < 100" using that by auto
-  \<bullet> x x y + < if \<medium_left_bracket>
-  \<nu>obtain z where c: "x < z" by auto \<medium_right_bracket>
-  finish
-
-
-proc add02: "(( x \<tycolon> \<nat>[32]) named x, y \<tycolon> \<nat>[32])" \<longmapsto> "(x + x + y \<tycolon> \<nat>[32])"
-if A[used]:"x < 100" and [used]:"y < 100"
-    \<bullet> x x y + +
-    \<nu>obtain z where c: "x < z" by auto
-  finish
-
-thm add2_\<nu>proc
-
-
-proc add3: "(x \<tycolon> \<nat>[32], y \<tycolon> \<nat>[32])" \<longmapsto> "(x + x + y \<tycolon> \<nat>[32])"
-  if [used]:"x < 100" and [used]:"y < 100"
-  \<bullet> x x y + +
-  \<nu>have gg: "x < 200"  by auto
-  finish
-thm add3_\<nu>proc
-
-thm add3_\<nu>proc
-
-
-
-
-thm add2_\<nu>proc
-
-ML \<open>map (Attrib.attribute @{context}) @{attributes [elim]}\<close>
 end
