NuSys.thy
@@ -257,7 +257,7 @@ end\<close>
 subsubsection \<open>Simplifiers & Resonings\<close>
 
 \<nu>processor \<nu>simplifier 40 \<open>\<^bold>c\<^bold>u\<^bold>r\<^bold>r\<^bold>e\<^bold>n\<^bold>t blk \<^bold>r\<^bold>e\<^bold>s\<^bold>u\<^bold>l\<^bold>t\<^bold>s \<^bold>i\<^bold>n T\<close>  \<open>NuProcessors.simplifier []\<close>
-\<nu>processor \<nu>simplifier_final 9999 \<open>PROP P\<close>  \<open>NuProcessors.simplifier []\<close>
+(* \<nu>processor \<nu>simplifier_final 9999 \<open>PROP P\<close>  \<open>NuProcessors.simplifier []\<close> *)
 
 \<nu>processor \<nu>resolver 9000 \<open>PROP P \<Longrightarrow> PROP Q\<close> \<open>fn ctx => fn meta => Scan.succeed (fn _ =>
   NuBasics.elim_SPEC meta |> apfst (fn major =>
